intermediate2/Zeta.Intermediate.StateRel.fst
@@ -1,0 +1,346 @@
+module Zeta.Intermediate.StateRel
+
+open FStar.Classical
+open Zeta.BinTree
+open Zeta.Key
+open Zeta.GenKey
+open Zeta.Record
+open Zeta.HashFunction
+
+let empty_store_rel
+  (vcfg: verifier_config)
+  : Lemma (ensures (empty_store vcfg `store_rel` HV.empty_store vcfg.app))
+  = let sts = empty_store vcfg in
+    let stk = HV.empty_store vcfg.app in
+
+    assert(is_map sts);
+    let aux (k:_)
+      : Lemma (ensures ((store_contains_key sts k = HV.store_contains stk k) /\
+                       (store_contains_key sts k ==>
+                       (let s = slot_of_key sts k in
+                       stored_key sts s = HV.stored_key stk k /\
+                       stored_value sts s = HV.stored_value stk k /\
+                       add_method_of sts s = HV.add_method_of stk k))))
+      = lemma_empty_contains_nokey #vcfg k;
+        assert(not (store_contains_key sts k));
+        assert(not (HV.store_contains stk k));
+        ()
+    in
+    forall_intro aux
+
+let lemma_empty_vtls_rel
+  (#vcfg: verifier_config)
+  (t:nat{t < vcfg.thread_count})
+  : Lemma (ensures (let vss = init_thread_state vcfg t in
+                    let vsk = HV.init_thread_state vcfg.app t in
+                    vtls_rel vss vsk))
+  = let vss = init_thread_state vcfg t in
+    let sts = vss.st in
+    let _sts = empty_store vcfg in
+    let vsk = HV.init_thread_state vcfg.app t in
+    let _stk = HV.empty_store vcfg.app in
+    let stk = vsk.st in
+    assert(vss.valid = vsk.valid /\ vss.tid = vsk.tid /\ vss.clock = vsk.clock);
+    empty_store_rel vcfg;
+    if t = 0 then
+      let aux (k:_)
+        : Lemma (ensures ((store_contains_key sts k = HV.store_contains stk k) /\
+                         (store_contains_key sts k ==>
+                         (let s = slot_of_key sts k in
+                         stored_key sts s = HV.stored_key stk k /\
+                         stored_value sts s = HV.stored_value stk k /\
+                         add_method_of sts s = HV.add_method_of stk k))))
+        = ()
+      in
+      forall_intro aux
+
+let lemma_runapp_simulates_spec
+      (#vcfg:_)
+      (vss:vtls_t vcfg{vss.valid})
+      (vsk:_ {vtls_rel vss vsk})
+      (e:logS_entry vcfg{GV.is_appfn e})
+  : Lemma (requires (valid_logS_entry vss e))
+          (ensures (let ek = to_logk_entry vss e in
+                    vtls_rel (GV.verify_step e vss) (GV.verify_step ek vsk)))
+  = admit()
+
+
+let amp (#vcfg:_) (vss:vtls_t vcfg {vss.valid}) (e: logS_entry vcfg {GV.AddM? e})
+  : addm_param vcfg
+  = let GV.AddM r s s' = e in
+    AMP s r s' vss
+
+#push-options "--fuel 0 --ifuel 1 --query_stats"
+
+let lemma_vaddm_preserves_spec_unrelatedkey
+  (#vcfg: verifier_config)
+  (vss: vtls_t vcfg {vss.valid})
+  (vsk: HV.vtls_t vcfg.app)
+  (e: logS_entry _ {GV.AddM? e})
+  (ki: base_key)
+  : Lemma (requires (let sts = vss.st in
+                     let a = amp vss e in
+                     addm_precond a /\
+                     vtls_rel vss vsk /\
+                     valid_logS_entry vss e /\
+                     not (store_contains_key sts (addm_base_key a)) /\
+                     ki <> addm_base_key a /\
+                     ki <> addm_anc_key a))
+          (ensures (let ek = to_logk_entry vss e in
+                    let vss_ = GV.verify_step e vss in
+                    let sts_ = vss_.st in
+                    let vsk_: HV.vtls_t vcfg.app = GV.verify_step ek vsk in
+                    let stk_ = vsk_.st in
+                    is_map sts_ /\
+                    store_rel_key sts_ stk_ ki))
+  = let sts = vss.st in
+    let a = amp vss e in
+    let stk = vsk.st in
+    let ek = to_logk_entry vss e in
+    let a = amp vss e in
+    let GV.AddM r s s' = e in
+
+    let k' = addm_anc_key a in
+    let k = addm_base_key a in
+
+    assert(GV.add_record ek = r);
+    assert(GV.add_slot ek = k);
+    assert(GV.ancestor_slot ek = k');
+
+    store_rel_slot sts stk s';
+    assert(HV.store_contains stk k');
+    assert(HV.stored_value stk k' = stored_value sts s');
+
+    let d = addm_dir a in
+    let vss_ = GV.verify_step e vss in
+    let sts_ = vss_.st in
+    let vsk_: HV.vtls_t vcfg.app = GV.verify_step ek vsk in
+    let stk_ = vsk_.st in
+
+    lemma_vaddm_preserves_ismap_new_key vss e;
+    assert(is_map sts_);
+
+    elim_key_store_rel sts stk ki;
+    if HV.store_contains stk ki then (
+      let si = slot_of_key sts ki in
+
+      (* si cannot be s or s' since the key stored there is ki *)
+      assert(stored_base_key sts si = ki);
+      assert(si <> s /\ si <> s');
+
+      lemma_addm_identical_except2 vss e si
+    )
+
+let lemma_vaddm_preserves_spec_key
+  (#vcfg: verifier_config)
+  (vss: vtls_t vcfg {vss.valid})
+  (vsk: HV.vtls_t vcfg.app)
+  (e: logS_entry _ {GV.AddM? e})
+  : Lemma (requires (let sts = vss.st in
+                     let a = amp vss e in
+                     addm_precond a /\
+                     vtls_rel vss vsk /\
+                     valid_logS_entry vss e /\
+                     not (store_contains_key sts (addm_base_key a))))
+          (ensures (let ek = to_logk_entry vss e in
+                    let vss_ = GV.verify_step e vss in
+                    let sts_ = vss_.st in
+                    let vsk_: HV.vtls_t vcfg.app = GV.verify_step ek vsk in
+                    let stk_ = vsk_.st in
+                    let a = amp vss e in
+                    let k = addm_base_key a in
+                    is_map sts_ /\
+                    store_rel_key sts_ stk_ k))
+  = lemma_vaddm_preserves_ismap_new_key vss e
+
+let lemma_vaddm_preserves_spec_anc_key
+  (#vcfg: verifier_config)
+  (vss: vtls_t vcfg {vss.valid})
+  (vsk: HV.vtls_t vcfg.app)
+  (e: logS_entry _ {GV.AddM? e})
+  : Lemma (requires (let sts = vss.st in
+                     let a = amp vss e in
+                     addm_precond a /\
+                     vtls_rel vss vsk /\
+                     valid_logS_entry vss e /\
+                     not (store_contains_key sts (addm_base_key a))))
+          (ensures (let ek = to_logk_entry vss e in
+                    let vss_ = GV.verify_step e vss in
+                    let sts_ = vss_.st in
+                    let vsk_: HV.vtls_t vcfg.app = GV.verify_step ek vsk in
+                    let stk_ = vsk_.st in
+                    let a = amp vss e in
+                    let k = addm_anc_key a in
+                    is_map sts_ /\
+                    store_rel_key sts_ stk_ k))
+  = lemma_vaddm_preserves_ismap_new_key vss e
+
+let lemma_vaddm_preserves_spec_case_valid
+  (#vcfg: verifier_config)
+  (vss: vtls_t vcfg {vss.valid})
+  (vsk: HV.vtls_t vcfg.app)
+  (e: logS_entry _ {GV.AddM? e})
+  : Lemma (requires (let sts = vss.st in
+                     let a = amp vss e in
+                     addm_precond a /\
+                     vtls_rel vss vsk /\
+                     valid_logS_entry vss e /\
+                     not (store_contains_key sts (addm_base_key a))))
+          (ensures (let ek = to_logk_entry vss e in
+                    let vss_ = GV.verify_step e vss in
+                    let vsk_: HV.vtls_t vcfg.app = GV.verify_step ek vsk in
+                    vtls_rel vss_ vsk_))
+  = let sts = vss.st in
+    let a = amp vss e in
+    let stk = vsk.st in
+    let ek = to_logk_entry vss e in
+    let a = amp vss e in
+    let GV.AddM r s s' = e in
+
+    let k' = addm_anc_key a in
+    let k = addm_base_key a in
+
+    assert(GV.add_record ek = r);
+    assert(GV.add_slot ek = k);
+    assert(GV.ancestor_slot ek = k');
+
+    store_rel_slot sts stk s';
+    assert(HV.store_contains stk k');
+    assert(HV.stored_value stk k' = stored_value sts s');
+
+    let d = addm_dir a in
+    let vss_ = GV.verify_step e vss in
+    let sts_ = vss_.st in
+    let vsk_: HV.vtls_t vcfg.app = GV.verify_step ek vsk in
+    let stk_ = vsk_.st in
+
+    lemma_vaddm_preserves_ismap_new_key vss e;
+    assert(is_map sts_);
+
+    assert(vss_.valid = vsk_.valid);
+    assert(vss_.clock = vsk_.clock);
+    assert(vss_.tid = vsk_.tid);
+
+    let aux (k2:_)
+      : Lemma (ensures (store_rel_key sts_ stk_ k2))
+      = if k2 = k then lemma_vaddm_preserves_spec_key vss vsk e
+        else if k2 = k' then lemma_vaddm_preserves_spec_anc_key vss vsk e
+        else lemma_vaddm_preserves_spec_unrelatedkey vss vsk e k2
+    in
+    forall_intro aux;
+    assert(store_rel sts_ stk_);
+    ()
+
+let lemma_vaddm_preserves_spec_case_fail
+  (#vcfg: verifier_config)
+  (vss: vtls_t vcfg {vss.valid})
+  (vsk: HV.vtls_t vcfg.app)
+  (e: logS_entry _ {GV.AddM? e})
+  : Lemma (requires (let sts = vss.st in
+                     let a = amp vss e in
+                     ~ (addm_precond a) /\
+                     vtls_rel vss vsk /\
+                     valid_logS_entry vss e /\
+                     not (store_contains_key sts (addm_base_key a)) /\
+                     slot_points_to_is_merkle_points_to sts))
+          (ensures (let ek = to_logk_entry vss e in
+                    let vss_ = GV.verify_step e vss in
+                    let vsk_: HV.vtls_t vcfg.app = GV.verify_step ek vsk in
+                    vtls_rel vss_ vsk_))
+  = let sts = vss.st in
+    let a = amp vss e in
+    let stk = vsk.st in
+    let ek = to_logk_entry vss e in
+    let a = amp vss e in
+    let GV.AddM r s s' = e in
+
+    (* otherwise e would not be a valid log entry *)
+    assert(empty_slot sts s /\ inuse_slot sts s');
+
+    let k = addm_base_key a in
+    let k' = stored_base_key sts s' in
+
+    elim_key_store_rel sts stk k';
+    lemma_ismap_correct sts s' (slot_of_key sts k');
+
+    if is_proper_desc k k' then (
+      assert(addm_precond1 a);
+
+      (* ancestor merkle value in intermediate *)
+      let mvs' = addm_anc_val_pre a in
+      let d = addm_dir a in
+
+      (* and it should be the same in spec *)
+      assert(HV.stored_value stk k' = IntV mvs');
+
+      if Merkle.points_to_none mvs' d then (
+
+        assert(addm_precond2 a /\ addm_anc_points_null a);
+
+        (* since a does not satisfy precond, one of these should hold *)
+        assert(not (is_init_record r) \/ points_to_some_slot sts s' d);
+
+        if is_init_record r then (
+          (* intermediate fails because s' points to some slot along addm direction *)
+          assert(points_to_some_slot sts s' d);
+
+          let s2 = pointed_slot sts s' d in
+          assert(slot_points_to_is_merkle_points_to_local sts s' s2 d);
+
+          (* which produces a contradiction since we have mv_points_none mvs' d *)
+          assert(False);
+          ()
+        )
+      )
+      else if Merkle.points_to mvs' d k then (
+        let _,gv = r in
+        assert(addm_precond2 a /\ addm_anc_points_to_key a);
+        assert(Merkle.desc_hash mvs' d <> Merkle.Desc k (hashfn gv) false \/
+               points_to_some_slot sts s' d);
+
+        if Merkle.desc_hash mvs' d = Merkle.Desc k (hashfn gv) false then (
+          let s2 = pointed_slot sts s' d in
+          assert(slot_points_to_is_merkle_points_to_local sts s' s2 d);
+          assert(stored_base_key sts s2 = k);
+          (* this imnplies s2 is in fact s, which is a contradiction (since s is inuse_slot then )*)
+          lemma_ismap_correct sts s s2;
+          assert(s = s2);
+
+          assert(False)
+        )
+      )
+    )
+
+#pop-options
+
+let lemma_vaddm_preserves_spec_new_key
+      (#vcfg:_)
+      (vs:vtls_t vcfg{vs.valid})
+      (vs':_ {vtls_rel vs vs'})
+      (e:logS_entry _{GV.AddM? e})
+  : Lemma (requires (let st = vs.st in
+                     let GV.AddM (gk,gv) _  _ = e in
+                     let k = to_base_key gk in
+                     valid_logS_entry vs e /\
+                     not (store_contains_key st k) /\
+                     slot_points_to_is_merkle_points_to st))
+          (ensures (let ek = to_logk_entry vs e in
+                    vtls_rel (GV.verify_step e vs) (GV.verify_step ek vs')))
+  = if (GV.verify_step e vs).valid then
+      lemma_vaddm_preserves_spec_case_valid vs vs' e
+    else
+      lemma_vaddm_preserves_spec_case_fail vs vs' e
+
+let lemma_vaddb_preserves_spec_new_key
+      (#vcfg:_)
+      (vs:vtls_t vcfg{vs.valid})
+      (vs':_ {vtls_rel vs vs'})
+      (e:logS_entry _{GV.AddB? e})
+  : Lemma (requires (let st = vs.st in
+                     let GV.AddB (gk,gv) _  _ _ = e in
+                     let k = to_base_key gk in
+                     valid_logS_entry vs e /\
+                     not (store_contains_key st k)))
+          (ensures (let ek = to_logk_entry vs e in
+                    vtls_rel (GV.verify_step e vs) (GV.verify_step ek vs')))
+  = admit()
